finish up to Equality case, and add new premises
that constructor names in the environment and store appear in the
constructor name environment. this is probably necessary for the
equality case, although i am currently cheating the final case of that
since the semantics doesn't guarantee no comparison of closures.

compiler/correctness/expToCexpScript.sml
@@ -402,11 +402,37 @@ val do_app_Opapp_SOME = store_thm("do_app_Opapp_SOME",
 
 (* correctness *)
 
-(*
-val v_to_Cv_inj_rwt = store_thm(
-"v_to_Cv_inj_rwt",
-``∀s v1 v2. (v_to_Cv s v1 = v_to_Cv s v2) = (v1 = v2)``,
-probably not true until equality is corrected in the source language *)
+val v_to_Cv_inj = store_thm(
+"v_to_Cv_inj",
+``(∀s (v1:α v) v2.
+    all_cns v1 ⊆ set (MAP FST cenv) ∧
+    all_cns v2 ⊆ set (MAP FST cenv) ∧
+    good_cenv (cenv:envC) ∧
+    good_cmap cenv s ∧
+    (*
+    no_closures v1 ∧ no_closures v2 ∧
+    *)
+    (v_to_Cv s v1 = v_to_Cv s v2) ⇒ (v1 = v2)) ∧
+  (∀s (vs1:α v list) vs2.
+    BIGUNION (IMAGE all_cns (set vs1)) ⊆ set (MAP FST cenv) ∧
+    BIGUNION (IMAGE all_cns (set vs2)) ⊆ set (MAP FST cenv) ∧
+    good_cenv cenv ∧
+    good_cmap cenv s ∧
+    (*
+    EVERY no_closures vs1 ∧ EVERY no_closures vs2 ∧
+    *)
+    (vs_to_Cvs s vs1 = vs_to_Cvs s vs2) ⇒ (vs1 = vs2)) ∧
+  (∀(s:string|->num) (env1:α envE).T)``,
+ho_match_mp_tac v_to_Cv_ind >> rw[v_to_Cv_def,LET_THM,vs_to_Cvs_MAP,env_to_Cenv_MAP] >>
+TRY (Cases_on`v2`>>fs[v_to_Cv_def,LET_THM]>>NO_TAC)
+>- (
+  Cases_on`v2`>>fs[v_to_Cv_def,vs_to_Cvs_MAP,MAP_EQ_EVERY2,EVERY2_EVERY,LET_THM] >>
+  fs[good_cenv_def,good_cmap_def,MEM_MAP,EXISTS_PROD] >>
+  metis_tac[] )
+>- cheat
+>- cheat
+>- (Cases_on`vs2`>>fs[]))
+
 
 (* TODO: categorise *)
 
@@ -618,10 +644,22 @@ val exp_to_Cexp_append_bvars_matchable = store_thm(
   qsuff_tac`z = s'`>-PROVE_TAC[]>>
   simp[exp_to_Cexp_state_component_equality,Abbr`z`])
 
+val closed_under_cenv_def = Define`
+  closed_under_cenv cenv env s =
+  (∀v. v ∈ env_range env ∨ MEM v s ⇒ all_cns v ⊆ set (MAP FST cenv))`
+
+val evaluate_closed_under_cenv = store_thm("evaluate_closed_under_cenv",
+  ``∀cenv s env exp res. closed_under_cenv cenv env s ∧ evaluate cenv s env exp res ⇒
+    closed_under_cenv cenv env (FST res)``,
+  rw[] >>
+  qspecl_then[`cenv`,`s`,`env`,`exp`,`res`]mp_tac (CONJUNCT1 evaluate_all_cns) >>
+  fsrw_tac[DNF_ss][closed_under_cenv_def])
+
 val exp_to_Cexp_thm1 = store_thm("exp_to_Cexp_thm1",
   ``(∀cenv s env exp res. evaluate cenv s env exp res ⇒
      FV exp ⊆ set (MAP FST env) ∧
      (EVERY closed s) ∧ (EVERY closed (MAP (FST o SND) env)) ∧
+     closed_under_cenv cenv env s ∧
      good_cenv cenv ∧ (SND res ≠ Rerr Rtype_error) ⇒
      ∀cm. good_cmap cenv cm ⇒
        ∃Cres.
@@ -635,6 +673,7 @@ val exp_to_Cexp_thm1 = store_thm("exp_to_Cexp_thm1",
     (∀cenv s env exps res. evaluate_list cenv s env exps res ⇒
      (BIGUNION (IMAGE FV (set exps)) ⊆ set (MAP FST env)) ∧
      (EVERY closed s) ∧ (EVERY closed (MAP (FST o SND) env)) ∧
+     closed_under_cenv cenv env s ∧
      good_cenv cenv ∧ (SND res ≠ Rerr Rtype_error) ⇒
      ∀cm. good_cmap cenv cm ⇒
        ∃Cres.
@@ -663,8 +702,11 @@ val exp_to_Cexp_thm1 = store_thm("exp_to_Cexp_thm1",
     last_x_assum(qspec_then`cm`mp_tac) >> simp[] >>
     disch_then(Q.X_CHOOSE_THEN`s2`strip_assume_tac) >>
     qspecl_then[`cenv`,`s`,`env`,`exp`,`(s',Rerr (Rraise (Int_error n)))`]mp_tac(CONJUNCT1 evaluate_closed) >>
-    fsrw_tac[DNF_ss][env_to_Cenv_MAP,SUBSET_DEF,lem] >> strip_tac >>
-    first_x_assum(qspec_then`cm`mp_tac) >> simp[] >>
+    qspecl_then[`cenv`,`s`,`env`,`exp`,`(s',Rerr (Rraise (Int_error n)))`]mp_tac(evaluate_closed_under_cenv) >>
+    fsrw_tac[DNF_ss][env_to_Cenv_MAP,SUBSET_DEF,lem] >> strip_tac >> strip_tac >>
+    first_x_assum(qspec_then`cm`mp_tac) >>
+    fsrw_tac[DNF_ss][closed_under_cenv_def,EXISTS_PROD] >>
+    disch_then(mp_tac o UNDISCH_ALL) >>
     disch_then(qx_choosel_then[`s3`,`v`]strip_assume_tac) >>
     CONV_TAC(RESORT_EXISTS_CONV List.rev) >>
     map_every qexists_tac[`n`,`s2`] >> simp[] >> fs[v_to_Cv_def] >>
@@ -764,6 +806,9 @@ val exp_to_Cexp_thm1 = store_thm("exp_to_Cexp_thm1",
       rw[Once(CONJUNCT2 Cevaluate_cases)] >> fsrw_tac[DNF_ss][] >>
       rw[Once(CONJUNCT2 Cevaluate_cases)] >> fsrw_tac[DNF_ss][] >>
       rpt (first_x_assum (qspec_then `cm` mp_tac)) >>
+      `closed_under_cenv cenv env' s'' ∧ closed_under_cenv cenv env s'` by (
+        `(s'' = s3) ∧ (env' = env)` by fs[do_app_Opn_SOME] >>
+        imp_res_tac evaluate_closed_under_cenv >> fs[] ) >>
       rw[] >>
       qmatch_assum_rename_tac `syneq FEMPTY FEMPTY (v_to_Cv cm v1) w1`[] >>
       qspecl_then[`cenv`,`s`,`env`,`e1`,`(s',Rval v1)`]mp_tac(CONJUNCT1 evaluate_closed) >>
@@ -797,8 +842,8 @@ val exp_to_Cexp_thm1 = store_thm("exp_to_Cexp_thm1",
         fs[i0_def] >>
         metis_tac[EVERY2_syneq_trans] ) >>
       simp[exp_to_Cexp_def] >> strip_tac >>
-      fs[v_to_Cv_def] >>
       conj_tac >- metis_tac[EVERY2_syneq_trans] >>
+      fs[v_to_Cv_def] >> rw[] >>
       Cases_on`opn`>>fs[]>>
       fs[v_to_Cv_def,opn_lookup_def,i0_def] >>
       Cases_on`n2=0`>>fs[v_to_Cv_def] )
@@ -814,6 +859,10 @@ val exp_to_Cexp_thm1 = store_thm("exp_to_Cexp_thm1",
       fs[] >>
       Q.ISPECL_THEN[`s2`,`s4`,`env`,`Opb opb`,`v1`,`v2`,`env'`,`exp''`]mp_tac do_app_closed >>
       simp[] >> strip_tac >> fs[] >>
+      `closed_under_cenv cenv env s1 ∧ closed_under_cenv cenv env' s4` by (
+        fs[do_app_Opb_SOME] >>
+        imp_res_tac evaluate_closed_under_cenv >> rfs[] ) >>
+      fs[] >>
       rpt (first_x_assum (qspec_then `cm` mp_tac)) >> rw[] >>
       qmatch_assum_rename_tac `syneq FEMPTY FEMPTY (v_to_Cv m v1) w1`[] >>
       qmatch_assum_rename_tac `syneq FEMPTY FEMPTY (v_to_Cv m v2) w2`[] >>
@@ -856,33 +905,30 @@ val exp_to_Cexp_thm1 = store_thm("exp_to_Cexp_thm1",
         map_every qexists_tac [`w1`,`sd`] >> fs[] >>
         rw[Once Cevaluate_cases] >>
         srw_tac[DNF_ss][] >>
-
-        qspecl_then[`FEMPTY`,`FEMPTY`,`sb`,`sd`,`enva`,`e2a`,`(se,Rval w2)`]mp_tac Cevaluate_any_syneq_store >>
-        fsrw_tac[DNF_ss][EXISTS_PROD] >>
-        qx_gen_tac`sf` >> qx_gen_tac`w3` >>
-        strip_tac >>
-        Q.PAT_ABBREV_TAC`fv = fresh_var X` >>
-        qspecl_then[`FEMPTY`,`FEMPTY`,`sd`,`enva`,`e2a`,`(sf,Rval w3)`,`fv`,`w1`]mp_tac Cevaluate_FUPDATE >>
-        `fv ∉ free_vars FEMPTY e2a` by (
-          unabbrev_all_tac >>
-          match_mp_tac fresh_var_not_in_any >>
-          rw[] ) >>
-        fsrw_tac[DNF_ss][EXISTS_PROD] >>
-        qx_gen_tac`sg`>>qx_gen_tac`w4`>>
-        strip_tac >>
+        qspecl_then[`FEMPTY`,`sb`,`enva`,`e2a`,`(se,Rval w2)`]mp_tac(CONJUNCT1 Cevaluate_syneq) >> simp[] >>
+        disch_then(qspecl_then[`FEMPTY`,`λv1 v2. v2 = v1 + 1`,`sd`,`w1::enva`,`shift 1 0 e2a`]mp_tac) >>
+        qmatch_abbrev_tac`(P⇒Q)⇒R` >>
+        `P` by (
+          map_every qunabbrev_tac[`P`,`Q`,`R`] >>
+          conj_tac >- (
+            simp[shift_def] >>
+            match_mp_tac mkshift_thm >>
+            simp[ADD1,Abbr`enva`,Abbr`e2a`,env_to_Cenv_MAP] >>
+            match_mp_tac free_vars_exp_to_Cexp_matchable >>
+            simp[] ) >>
+          lrw[EL_CONS,PRE_SUB1] ) >>
+        simp[] >> map_every qunabbrev_tac[`P`,`Q`,`R`] >> pop_assum kall_tac >>
+        fsrw_tac[DNF_ss][FORALL_PROD] >>
+        map_every qx_gen_tac[`sf`,`w3`] >> strip_tac >>
         CONV_TAC (RESORT_EXISTS_CONV List.rev) >>
-        map_every qexists_tac [`w4`,`sg`] >> fs[] >>
+        map_every qexists_tac [`w3`,`sf`] >> fs[] >>
         rw[Once Cevaluate_cases] >>
         srw_tac[DNF_ss][] >>
         rw[Once (CONJUNCT2 Cevaluate_cases)] >>
         rw[Once (CONJUNCT2 Cevaluate_cases)] >>
-        rw[Once (CONJUNCT2 Cevaluate_cases)] >>
-        rw[FAPPLY_FUPDATE_THM,NOT_fresh_var] >>
-        map_every qunabbrev_tac[`w1`,`w2`] >> rw[] >>
-        fs[Q.SPECL[`FEMPTY`,`CLitv l`]syneq_cases] >> rw[] >>
-        fs[Q.SPECL[`FEMPTY`,`CLitv l`]syneq_cases] >> rw[] >>
-        rw[integerTheory.int_gt] >>
-        metis_tac[fmap_rel_syneq_trans])
+        lrw[Once (CONJUNCT2 Cevaluate_cases),ADD1,Abbr`w1`,Abbr`w2`] >>
+        fs[] >> rw[integerTheory.int_gt] >>
+        metis_tac[EVERY2_syneq_trans])
       >- (
         rw[Once Cevaluate_cases] >>
         srw_tac[DNF_ss][] >>
@@ -896,19 +942,14 @@ val exp_to_Cexp_thm1 = store_thm("exp_to_Cexp_thm1",
         rw[Once (CONJUNCT2 Cevaluate_cases)] >>
         srw_tac[DNF_ss][] >>
         CONV_TAC (RESORT_EXISTS_CONV List.rev) >>
-        qexists_tac`sd`>>
-        qexists_tac`w2`>>
-        qexists_tac`w1`>>
-        qspecl_then[`FEMPTY`,`FEMPTY`,`sb`,`sd`,`enva`,`e2a`,`(se,Rval w2)`]mp_tac(Cevaluate_any_syneq_store) >>
-        fsrw_tac[DNF_ss][EXISTS_PROD,Abbr`w2`,Abbr`w1`] >>
-        qx_gen_tac`sf` >>
-        qx_gen_tac`w3` >>
-        strip_tac >>
-        fs[Q.SPECL[`FEMPTY`,`CLitv l`]syneq_cases] >>
-        `fmap_rel (syneq FEMPTY) sc sf` by PROVE_TAC[fmap_rel_syneq_trans] >>
+        map_every qexists_tac[`sd`,`w2`,`w1`] >>
+        qspecl_then[`FEMPTY`,`sb`,`enva`,`e2a`,`(se,Rval w2)`]mp_tac(CONJUNCT1 Cevaluate_syneq) >> simp[] >>
+        disch_then(qspecl_then[`FEMPTY`,`$=`,`sd`,`enva`,`e2a`]mp_tac) >> simp[syneq_exp_refl] >>
+        fsrw_tac[DNF_ss][FORALL_PROD,Abbr`w2`,Abbr`w1`] >>
+        qx_gen_tac`sf` >> strip_tac >>
         qexists_tac`sf`>>
-        rw[CompileTheory.i1_def] >>
-        ARITH_TAC )
+        reverse conj_tac >- metis_tac[EVERY2_syneq_trans] >>
+        rw[CompileTheory.i1_def] >> ARITH_TAC )
       >- (
         rw[Once Cevaluate_cases] >>
         srw_tac[DNF_ss][] >>
@@ -916,39 +957,35 @@ val exp_to_Cexp_thm1 = store_thm("exp_to_Cexp_thm1",
         map_every qexists_tac [`w1`,`sd`] >> fs[] >>
         rw[Once Cevaluate_cases] >>
         srw_tac[DNF_ss][] >>
-        qspecl_then[`FEMPTY`,`FEMPTY`,`sb`,`sd`,`enva`,`e2a`,`(se,Rval w2)`]mp_tac Cevaluate_any_syneq_store >>
-        fsrw_tac[DNF_ss][EXISTS_PROD] >>
-        qx_gen_tac`sf` >> qx_gen_tac`w3` >>
-        strip_tac >>
-        Q.PAT_ABBREV_TAC`fv = fresh_var X` >>
-        qspecl_then[`FEMPTY`,`FEMPTY`,`sd`,`enva`,`e2a`,`(sf,Rval w3)`,`fv`,`w1`]mp_tac Cevaluate_FUPDATE >>
-        `fv ∉ free_vars FEMPTY e2a` by (
-          unabbrev_all_tac >>
-          match_mp_tac fresh_var_not_in_any >>
-          rw[] ) >>
-        fsrw_tac[DNF_ss][EXISTS_PROD] >>
-        qx_gen_tac`sg`>>qx_gen_tac`w4`>>
-        strip_tac >>
+        qspecl_then[`FEMPTY`,`sb`,`enva`,`e2a`,`(se,Rval w2)`]mp_tac(CONJUNCT1 Cevaluate_syneq) >> simp[] >>
+        disch_then(qspecl_then[`FEMPTY`,`λv1 v2. v2 = v1 + 1`,`sd`,`w1::enva`,`shift 1 0 e2a`]mp_tac) >>
+        qmatch_abbrev_tac`(P⇒Q)⇒R` >>
+        `P` by (
+          map_every qunabbrev_tac[`P`,`Q`,`R`] >>
+          conj_tac >- (
+            simp[shift_def] >>
+            match_mp_tac mkshift_thm >>
+            simp[ADD1,Abbr`enva`,Abbr`e2a`,env_to_Cenv_MAP] >>
+            match_mp_tac free_vars_exp_to_Cexp_matchable >>
+            simp[] ) >>
+          lrw[EL_CONS,PRE_SUB1] ) >>
+        simp[] >> map_every qunabbrev_tac[`P`,`Q`,`R`] >> pop_assum kall_tac >>
+        fsrw_tac[DNF_ss][FORALL_PROD] >>
+        map_every qx_gen_tac[`sf`,`w3`] >> strip_tac >>
         CONV_TAC (RESORT_EXISTS_CONV List.rev) >>
-        map_every qexists_tac [`w4`,`sg`] >> fs[] >>
+        map_every qexists_tac [`w3`,`sf`] >> fs[] >>
         rw[Once Cevaluate_cases] >>
         srw_tac[DNF_ss][] >>
         rw[Once (CONJUNCT2 Cevaluate_cases)] >>
         rw[Once (CONJUNCT2 Cevaluate_cases)] >>
-        rw[Once (CONJUNCT2 Cevaluate_cases)] >>
-        rw[FAPPLY_FUPDATE_THM,NOT_fresh_var] >>
+        lrw[Once (CONJUNCT2 Cevaluate_cases),ADD1,Abbr`w1`,Abbr`w2`] >>
         rw[Once Cevaluate_cases] >>
         rw[Once (CONJUNCT2 Cevaluate_cases)] >>
         rw[Once (CONJUNCT2 Cevaluate_cases)] >>
         rw[Once (CONJUNCT2 Cevaluate_cases)] >>
-        srw_tac[DNF_ss][] >>
-        rw[FAPPLY_FUPDATE_THM,NOT_fresh_var] >>
-        map_every qunabbrev_tac[`w1`,`w2`] >> rw[] >>
-        fs[Q.SPECL[`FEMPTY`,`CLitv l`]syneq_cases] >> rw[] >>
-        `fmap_rel (syneq FEMPTY) sc sg` by PROVE_TAC[fmap_rel_syneq_trans] >>
-        fs[Q.SPECL[`FEMPTY`,`CLitv l`]syneq_cases] >> rw[] >>
-        rw[CompileTheory.i1_def] >>
-        ARITH_TAC) )
+        fs[] >>
+        lrw[ADD1,CompileTheory.i1_def] >- ARITH_TAC >>
+        metis_tac[EVERY2_syneq_trans]) )
     >- (
       rw[Once Cevaluate_cases] >>
       srw_tac[DNF_ss][] >>
@@ -956,74 +993,55 @@ val exp_to_Cexp_thm1 = store_thm("exp_to_Cexp_thm1",
       rw[Once(CONJUNCT2 Cevaluate_cases)] >>
       rw[Once(CONJUNCT2 Cevaluate_cases)] >>
       rw[Once(CONJUNCT2 Cevaluate_cases)] >>
-      srw_tac[DNF_ss][] >>
-      fs[] >>
+      srw_tac[DNF_ss][] >> fs[] >>
       qspecl_then[`cenv`,`s`,`env`,`e1`,`(s',Rval v1)`]mp_tac(CONJUNCT1 evaluate_closed) >>
       simp[]>>strip_tac >>
       qspecl_then[`cenv`,`s'`,`env`,`e2`,`(s3,Rval v2)`]mp_tac(CONJUNCT1 evaluate_closed) >>
       simp[]>>strip_tac >>
       Q.ISPECL_THEN[`s3`,`s''`,`env`,`Equality`,`v1`,`v2`,`env'`,`exp''`]mp_tac do_app_closed >>
-      simp[]>>strip_tac>>
-      fs[] >>
+      simp[]>>strip_tac>> fs[] >>
+      `closed_under_cenv cenv env' s'' ∧ closed_under_cenv cenv env s'` by (
+        fs[do_app_def] >> imp_res_tac evaluate_closed_under_cenv >> rfs[] ) >> fs[] >>
       rpt (first_x_assum (qspec_then `cm` mp_tac)) >>
       rw[EXISTS_PROD] >>
-      qmatch_assum_rename_tac `syneq FEMPTY(v_to_Cv cm v1) w1`[] >>
-      qmatch_assum_rename_tac `syneq FEMPTY(v_to_Cv m v2) w2`[] >>
-      qabbrev_tac`sa = store_to_Cstore m s` >>
-      qabbrev_tac`sb = store_to_Cstore m s'` >>
-      qabbrev_tac`sc = store_to_Cstore m s3` >>
-      qmatch_assum_abbrev_tac`Cevaluate FEMPTY FEMPTY sa enva e1a X` >>
-      qmatch_assum_rename_tac`Abbrev(X=(sd,Rval w1))`[]>>
-      qunabbrev_tac`X` >>
-      qmatch_assum_abbrev_tac`Cevaluate FEMPTY FEMPTY sb enva e2a X` >>
+      qmatch_assum_rename_tac `syneq FEMPTY FEMPTY(v_to_Cv cm v1) w1`[] >>
+      qmatch_assum_rename_tac `syneq FEMPTY FEMPTY(v_to_Cv m v2) w2`[] >>
+      qabbrev_tac`sa = MAP (v_to_Cv m) s` >>
+      qabbrev_tac`sb = MAP (v_to_Cv m) s'` >>
+      qabbrev_tac`sc = MAP (v_to_Cv m) s3` >>
+      qmatch_assum_abbrev_tac`Cevaluate FEMPTY sa enva e1a X` >>
+      qmatch_assum_rename_tac`Abbrev(X=(sd,Rval w1))`[]>> qunabbrev_tac`X` >>
+      qmatch_assum_abbrev_tac`Cevaluate FEMPTY sb enva e2a X` >>
       qmatch_assum_rename_tac`Abbrev(X=(se,Rval w2))`[]>>
-      qspecl_then[`FEMPTY`,`FEMPTY`,`sb`,`sd`,`enva`,`e2a`,`X`]mp_tac Cevaluate_any_syneq_store >>
-      `∀v. v ∈ FRANGE enva ⇒ Cclosed FEMPTY v` by (
-        unabbrev_all_tac >>
-        match_mp_tac IN_FRANGE_alist_to_fmap_suff >>
-        simp[env_to_Cenv_MAP,MAP_MAP_o,combinTheory.o_DEF,MEM_MAP,EXISTS_PROD] >>
-        srw_tac[DNF_ss][] >>
-        match_mp_tac (CONJUNCT1 v_to_Cv_closed) >>
-        fs[EVERY_MEM,EXISTS_PROD,MEM_MAP] >>
-        metis_tac[] ) >>
-      `free_vars FEMPTY e1a ⊆ FDOM enva` by (
-        unabbrev_all_tac >>
-        fsrw_tac[DNF_ss][SUBSET_DEF,env_to_Cenv_MAP,MEM_MAP,
-                         EXISTS_PROD,FORALL_PROD] ) >>
-      `free_vars FEMPTY e2a ⊆ FDOM enva` by (
-        unabbrev_all_tac >>
-        fsrw_tac[DNF_ss][SUBSET_DEF,env_to_Cenv_MAP,MEM_MAP,
-                         EXISTS_PROD,FORALL_PROD] ) >>
-      `∀v. v ∈ FRANGE sa ⇒ Cclosed FEMPTY v` by (
-        unabbrev_all_tac >>
-        simp[FRANGE_store_to_Cstore,MEM_MAP] >>
-        srw_tac[DNF_ss][] >>
-        match_mp_tac (CONJUNCT1 v_to_Cv_closed) >>
-        fs[EVERY_MEM] ) >>
-      `∀v. v ∈ FRANGE sb ⇒ Cclosed FEMPTY v` by (
-        unabbrev_all_tac >>
-        simp[FRANGE_store_to_Cstore,MEM_MAP] >>
-        srw_tac[DNF_ss][] >>
-        match_mp_tac (CONJUNCT1 v_to_Cv_closed) >>
-        fs[EVERY_MEM] ) >>
-      qspecl_then[`FEMPTY`,`FEMPTY`,`sa`,`enva`,`e1a`,`(sd,Rval w1)`]mp_tac(CONJUNCT1 Cevaluate_closed) >>
-      simp[] >> strip_tac >>
-      qspecl_then[`FEMPTY`,`FEMPTY`,`sb`,`enva`,`e2a`,`X`]mp_tac(CONJUNCT1 Cevaluate_closed) >>
-      simp[Abbr`X`] >> strip_tac >>
-      fsrw_tac[DNF_ss][EXISTS_PROD,FORALL_PROD] >>
-      map_every qx_gen_tac[`sf`,`w3`] >>
-      strip_tac >>
+      qspecl_then[`FEMPTY`,`sb`,`enva`,`e2a`,`X`]mp_tac(CONJUNCT1 Cevaluate_syneq) >> simp[] >>
+      disch_then(qspecl_then[`FEMPTY`,`$=`,`sd`,`enva`,`e2a`]mp_tac) >> simp[syneq_exp_refl] >>
+      fsrw_tac[DNF_ss][EXISTS_PROD,FORALL_PROD,Abbr`X`] >>
+      map_every qx_gen_tac[`sf`,`w3`] >> strip_tac >>
       map_every qexists_tac[`sf`,`w1`,`w3`,`sd`] >>
       simp[] >>
       fs[do_app_def] >>
       rpt BasicProvers.VAR_EQ_TAC >>
       fs[] >>
       rpt BasicProvers.VAR_EQ_TAC >>
-      fs[v_to_Cv_def,Q.SPECL[`c`,`CLitv l`]syneq_cases] >>
-      fs[exp_to_Cexp_def] >>
-      `fmap_rel (syneq FEMPTY) sc sf` by PROVE_TAC[fmap_rel_syneq_trans] >>
+      fs[v_to_Cv_def] >> fs[exp_to_Cexp_def] >>
+      conj_tac >- metis_tac[EVERY2_syneq_trans] >>
+      BasicProvers.CASE_TAC >- (
+        fs[] >>
+        `no_closures w2` by metis_tac[syneq_no_closures] >>
+        `w3 = w2` by metis_tac[no_closures_syneq_equal] >>
+        `w2 = v_to_Cv m v2` by metis_tac[no_closures_syneq_equal,syneq_no_closures] >>
+        `w1 = v_to_Cv m v1` by metis_tac[no_closures_syneq_equal,syneq_no_closures] >>
+        rw[] >>
+        reverse EQ_TAC >- rw[] >>
+        strip_tac >>
+        match_mp_tac (MP_CANON(CONJUNCT1 v_to_Cv_inj)) >>
+        qexists_tac`m` >>
+        qspecl_then[`cenv`,`s`,`env`,`e1`,`(s',Rval v1)`]mp_tac(CONJUNCT1 evaluate_all_cns) >>
+        qspecl_then[`cenv`,`s'`,`env`,`e2`,`(s'',Rval v2)`]mp_tac(CONJUNCT1 evaluate_all_cns) >>
+        fsrw_tac[DNF_ss][closed_under_cenv_def] ) >>
       cheat )
     >- (
+
       rw[Once Cevaluate_cases] >>
       srw_tac[DNF_ss][] >>
       disj1_tac >>
